$$
\frac{\theta^{n+1} - \theta^n}{\Delta t} + \mathcal{L}(\theta^{n+1}) + \frac{\mathcal{N}(\theta^n)}{\exp(I(\theta^n))} r^{n+1} - \mathcal{L}(\theta^n) = 0 \\
\frac{r^{n+1} - r^n}{\Delta t} = \exp(I(\theta^n))\cdot \left( \mathcal{N(\theta^{n}), \frac{\theta^{n+1} - \theta^{n}}{\Delta t}}\right)
$$

$$
\frac{\theta^{n+1} - \theta^n}{\Delta t} + \mathcal{L}(\theta^{n+1}) + \frac{C\cdot\mathcal{N}(\theta^n)}{\exp(I(\theta^n))} r^{n+1} - \mathcal{L}(\theta^n) = 0 \\
\frac{r^{n+1} - r^n}{\Delta t} = \frac{\exp(I(\theta^n))}{C}\cdot \left( \mathcal{N(\theta^{n}), \frac{\theta^{n+1} - \theta^{n}}{\Delta t}}\right)
$$

​	$\alpha = \dfrac{1}{\Delta t} + \lambda$





a,w - > loss 最小

y^

y = ax / 1000

y = ax 